04_Earley_Recognizer.thy
@@ -1,12 +1,589 @@
 (*<*)
 theory "04_Earley_Recognizer"
   imports
-    "../Examples"
+    "03_Fixpoint_Earley_Recognizer"
     "HOL-Library.LaTeXsugar"
 begin
 (*>*)
 
-chapter\<open>Earley Recogniser\<close>
+chapter\<open>Earley Recogniser Implementation\<close>
+
+section\<open>Definitions\<close>
+
+fun filter_with_index' :: "nat \<Rightarrow> ('a \<Rightarrow> bool) \<Rightarrow> 'a list \<Rightarrow> ('a \<times> nat) list" where
+  "filter_with_index' _ _ [] = []"
+| "filter_with_index' i P (x#xs) = (
+    if P x then (x,i) # filter_with_index' (i+1) P xs
+    else filter_with_index' (i+1) P xs)"
+
+definition filter_with_index :: "('a \<Rightarrow> bool) \<Rightarrow> 'a list \<Rightarrow> ('a \<times> nat) list" where
+  "filter_with_index P xs = filter_with_index' 0 P xs"
+
+datatype pointer =
+  Null
+  | Pre nat
+  | PreRed "nat \<times> nat \<times> nat" "(nat \<times> nat \<times> nat) list"
+
+datatype 'a entry =
+  Entry         
+  (item : "'a item")
+  (pointer : pointer)
+
+type_synonym 'a bin = "'a entry list"
+type_synonym 'a bins = "'a bin list"
+
+definition items :: "'a bin \<Rightarrow> 'a item list" where
+  "items b = map item b"
+
+definition pointers :: "'a bin \<Rightarrow> pointer list" where
+  "pointers b = map pointer b"
+
+definition bins_eq_items :: "'a bins \<Rightarrow> 'a bins \<Rightarrow> bool" where
+  "bins_eq_items bs0 bs1 \<longleftrightarrow> map items bs0 = map items bs1"
+
+definition bins_items :: "'a bins \<Rightarrow> 'a items" where
+  "bins_items bs = \<Union> { set (items (bs ! k)) | k. k < length bs }"
+
+definition bin_items_upto :: "'a bin \<Rightarrow> nat \<Rightarrow> 'a items" where
+  "bin_items_upto b i = { items b ! j | j. j < i \<and> j < length (items b) }"
+
+definition bins_items_upto :: "'a bins \<Rightarrow> nat \<Rightarrow> nat \<Rightarrow> 'a items" where
+  "bins_items_upto bs k i = \<Union> { set (items (bs ! l)) | l. l < k } \<union> bin_items_upto (bs ! k) i"
+
+definition wf_bin_items :: "'a cfg \<Rightarrow> 'a sentence \<Rightarrow> nat \<Rightarrow> 'a item list \<Rightarrow> bool" where
+  "wf_bin_items cfg inp k xs = (\<forall>x \<in> set xs. wf_item cfg inp x \<and> item_end x = k)"
+
+definition wf_bin :: "'a cfg \<Rightarrow> 'a sentence \<Rightarrow> nat \<Rightarrow> 'a bin \<Rightarrow> bool" where
+  "wf_bin cfg inp k b \<longleftrightarrow> distinct (items b) \<and> wf_bin_items cfg inp k (items b)"
+
+definition wf_bins :: "'a cfg \<Rightarrow> 'a list \<Rightarrow> 'a bins \<Rightarrow> bool" where
+  "wf_bins cfg inp bs \<longleftrightarrow> (\<forall>k < length bs. wf_bin cfg inp k (bs ! k))"
+
+definition nonempty_derives :: "'a cfg \<Rightarrow> bool" where
+  "nonempty_derives cfg = (\<forall>N. N \<in> set (\<NN> cfg) \<longrightarrow> \<not> derives cfg [N] [])"
+
+definition Init_it :: "'a cfg \<Rightarrow> 'a sentence \<Rightarrow> 'a bins" where
+  "Init_it cfg inp = (
+    let rs = filter (\<lambda>r. rule_head r = \<SS> cfg) (\<RR> cfg) in
+    let b0 = map (\<lambda>r. (Entry (init_item r 0) Null)) rs in
+    let bs = replicate (length inp + 1) ([]) in
+    bs[0 := b0])"
+
+definition Scan_it :: "nat \<Rightarrow> 'a sentence \<Rightarrow> 'a  \<Rightarrow> 'a item \<Rightarrow> nat \<Rightarrow> 'a entry list" where
+  "Scan_it k inp a x pre = (
+    if inp!k = a then
+      let x' = inc_item x (k+1) in
+      [Entry x' (Pre pre)]
+    else [])"
+
+definition Predict_it :: "nat \<Rightarrow> 'a cfg \<Rightarrow> 'a \<Rightarrow> 'a entry list" where
+  "Predict_it k cfg X = (
+    let rs = filter (\<lambda>r. rule_head r = X) (\<RR> cfg) in
+    map (\<lambda>r. (Entry (init_item r k) Null)) rs)"
+
+definition Complete_it :: "nat \<Rightarrow> 'a item \<Rightarrow> 'a bins \<Rightarrow> nat \<Rightarrow> 'a entry list" where
+  "Complete_it k y bs red = (
+    let orig = bs ! (item_origin y) in
+    let is = filter_with_index (\<lambda>x. next_symbol x = Some (item_rule_head y)) (items orig) in
+    map (\<lambda>(x, pre). (Entry (inc_item x k) (PreRed (item_origin y, pre, red) []))) is)"
+
+fun bin_upd :: "'a entry \<Rightarrow> 'a bin \<Rightarrow> 'a bin" where
+  "bin_upd e' [] = [e']"
+| "bin_upd e' (e#es) = (
+    case (e', e) of
+      (Entry x (PreRed px xs), Entry y (PreRed py ys)) \<Rightarrow> 
+        if x = y then Entry x (PreRed py (px#xs@ys)) # es
+        else e # bin_upd e' es
+      | _ \<Rightarrow> 
+        if item e' = item e then e # es
+        else e # bin_upd e' es)"
+
+fun bin_upds :: "'a entry list \<Rightarrow> 'a bin \<Rightarrow> 'a bin" where
+  "bin_upds [] b = b"
+| "bin_upds (e#es) b = bin_upds es (bin_upd e b)"
+
+definition bins_upd :: "'a bins \<Rightarrow> nat \<Rightarrow> 'a entry list \<Rightarrow> 'a bins" where
+  "bins_upd bs k es = bs[k := bin_upds es (bs!k)]"
+
+partial_function (tailrec) \<pi>_it' :: "nat \<Rightarrow> 'a cfg \<Rightarrow> 'a sentence \<Rightarrow> 'a bins \<Rightarrow> nat \<Rightarrow> 'a bins" where
+  "\<pi>_it' k cfg inp bs i = (
+    if i \<ge> length (items (bs ! k)) then bs
+    else
+      let x = items (bs!k) ! i in
+      let bs' =
+        case next_symbol x of
+          Some a \<Rightarrow>
+            if is_terminal cfg a then
+              if k < length inp then bins_upd bs (k+1) (Scan_it k inp a x i)
+              else bs
+            else bins_upd bs k (Predict_it k cfg a)
+        | None \<Rightarrow> bins_upd bs k (Complete_it k x bs i)
+      in \<pi>_it' k cfg inp bs' (i+1))"
+
+definition \<pi>_it :: "nat \<Rightarrow> 'a cfg \<Rightarrow> 'a sentence \<Rightarrow> 'a bins \<Rightarrow> 'a bins" where
+  "\<pi>_it k cfg inp bs = \<pi>_it' k cfg inp bs 0"
+
+fun \<I>_it :: "nat \<Rightarrow> 'a cfg \<Rightarrow> 'a sentence \<Rightarrow> 'a bins" where
+  "\<I>_it 0 cfg inp = \<pi>_it 0 cfg inp (Init_it cfg inp)"
+| "\<I>_it (Suc n) cfg inp = \<pi>_it (Suc n) cfg inp (\<I>_it n cfg inp)"
+
+definition \<II>_it :: "'a cfg \<Rightarrow> 'a sentence \<Rightarrow> 'a bins" where
+  "\<II>_it cfg inp = \<I>_it (length inp) cfg inp"
+
+section \<open>Wellformedness\<close>
+
+lemma distinct_bin_upd:
+  "distinct (items b) \<Longrightarrow> distinct (items (bin_upd e b))"
+(*<*)
+  sorry
+(*>*)
+
+lemma distinct_bin_upds:
+  "distinct (items b)  \<Longrightarrow> distinct (items (bin_upds es b))"
+(*<*)
+  sorry
+(*>*)
+
+lemma distinct_bins_upd:
+  "distinct (items (bs ! k)) \<Longrightarrow> distinct (items (bins_upd bs k ips ! k))"
+(*<*)
+  sorry
+(*>*)
+
+lemma distinct_Scan_it:
+  "distinct (items (Scan_it k inp a x pre))"
+  sorry
+
+lemma distinct_Predict_it:
+  "wf_cfg cfg \<Longrightarrow> distinct (items (Predict_it k cfg X))"
+(*<*)
+  sorry
+(*>*)
+
+lemma distinct_Complete_it:
+  assumes "wf_bins cfg inp bs" "item_origin y < length bs"
+  shows "distinct (items (Complete_it k y bs red))"
+(*<*)
+  sorry
+(*>*)
+
+lemma wf_bin_bin_upd:
+  assumes "wf_bin cfg inp k b" "wf_item cfg inp (item e) \<and> item_end (item e) = k"
+  shows "wf_bin cfg inp k (bin_upd e b)"
+(*<*)
+  sorry
+(*>*)
+
+lemma wf_bin_bin_upds:
+  assumes "wf_bin cfg inp k b" "distinct (items es)"
+  assumes "\<forall>x \<in> set (items es). wf_item cfg inp x \<and> item_end x = k"
+  shows "wf_bin cfg inp k (bin_upds es b)"
+(*<*)
+  sorry
+(*>*)
+
+lemma wf_bins_bins_upd:
+  assumes "wf_bins cfg inp bs" "distinct (items es)"
+  assumes "\<forall>x \<in> set (items es). wf_item cfg inp x \<and> item_end x = k"
+  shows "wf_bins cfg inp (bins_upd bs k es)"
+(*<*)
+  sorry
+(*>*)
+
+lemma wf_bins_Init_it:
+  assumes "wf_cfg cfg"
+  shows "wf_bins cfg inp (Init_it cfg inp)"
+(*<*)
+  sorry
+(*>*)
+
+lemma wf_bins_Scan_it:
+  assumes "wf_bins cfg inp bs" "k < length bs" "x \<in> set (items (bs ! k))" "k < length inp" "next_symbol x \<noteq> None"
+  shows "\<forall>y \<in> set (items (Scan_it k inp a x pre)). wf_item cfg inp y \<and> item_end y = (k+1)"
+(*<*)
+  sorry
+(*>*)
+
+lemma wf_bins_Predict_it:
+  assumes "wf_bins cfg inp bs" "k < length bs" "k \<le> length inp" "wf_cfg cfg"
+  shows "\<forall>y \<in> set (items (Predict_it k cfg X)). wf_item cfg inp y \<and> item_end y = k"
+(*<*)
+  sorry
+(*>*)
+
+lemma wf_bins_Complete_it:
+  assumes "wf_bins cfg inp bs" "k < length bs" "y \<in> set (items (bs ! k))"
+  shows "\<forall>x \<in> set (items (Complete_it k y bs red)). wf_item cfg inp x \<and> item_end x = k"
+(*<*)
+  sorry
+(*>*)
+
+
+definition wellformed_bins :: "(nat \<times> 'a cfg \<times> 'a sentence \<times> 'a bins) set" where
+  "wellformed_bins = { 
+    (k, cfg, inp, bs) | k cfg inp bs.
+      k \<le> length inp \<and>
+      length bs = length inp + 1 \<and>
+      wf_cfg cfg \<and>
+      wf_bins cfg inp bs
+  }"
+
+typedef 'a wf_bins = "wellformed_bins::(nat \<times> 'a cfg \<times> 'a sentence \<times> 'a bins) set"
+ (*<*)
+  sorry
+ (*>*)
+
+lemma wellformed_bins_Init_it:
+  assumes "k \<le> length inp" "wf_cfg cfg"
+  shows "(k, cfg, inp, Init_it cfg inp) \<in> wellformed_bins"
+(*<*)
+  sorry
+(*>*)
+
+lemma wellformed_bins_Complete_it:
+  assumes "(k, cfg, inp, bs) \<in> wellformed_bins" "\<not> length (items (bs ! k)) \<le> i"
+  assumes "x = items (bs ! k) ! i" "next_symbol x = None"
+  shows "(k, cfg, inp, bins_upd bs k (Complete_it k x bs red)) \<in> wellformed_bins"
+(*<*)
+  sorry
+(*>*)
+
+lemma wellformed_bins_Scan_it:
+  assumes "(k, cfg, inp, bs) \<in> wellformed_bins" "\<not> length (items (bs ! k)) \<le> i"
+  assumes "x = items (bs ! k) ! i" "next_symbol x = Some a"
+  assumes "is_terminal cfg a" "k < length inp"
+  shows "(k, cfg, inp, bins_upd bs (k+1) (Scan_it k inp a x pre)) \<in> wellformed_bins"
+(*<*)
+  sorry
+(*>*)
+
+lemma wellformed_bins_Predict_it:
+  assumes "(k, cfg, inp, bs) \<in> wellformed_bins" "\<not> length (items (bs ! k)) \<le> i"
+  assumes "x = items (bs ! k) ! i" "next_symbol x = Some a" "\<not> is_terminal cfg a"
+  shows "(k, cfg, inp, bins_upd bs k (Predict_it k cfg a)) \<in> wellformed_bins"
+(*<*)
+  sorry
+(*>*)
+
+fun earley_measure :: "nat \<times> 'a cfg \<times> 'a sentence \<times> 'a bins \<Rightarrow> nat \<Rightarrow> nat" where
+  "earley_measure (k, cfg, inp, bs) i = card { x | x. wf_item cfg inp x \<and> item_end x = k } - i"
+
+lemma \<pi>_it'_induct:
+  assumes "(k, cfg, inp, bs) \<in> wellformed_bins"
+  assumes base: "\<And>k cfg inp bs i. i \<ge> length (items (bs ! k)) \<Longrightarrow> P k cfg inp bs i"
+  assumes complete: "\<And>k cfg inp bs i x. \<not> i \<ge> length (items (bs ! k)) \<Longrightarrow> x = items (bs ! k) ! i \<Longrightarrow>
+            next_symbol x = None \<Longrightarrow> P k cfg inp (bins_upd bs k (Complete_it k x bs i)) (i+1) \<Longrightarrow> P k cfg inp bs i"
+  assumes scan: "\<And>k cfg inp bs i x a. \<not> i \<ge> length (items (bs ! k)) \<Longrightarrow> x = items (bs ! k) ! i \<Longrightarrow>
+            next_symbol x = Some a \<Longrightarrow> is_terminal cfg a \<Longrightarrow> k < length inp \<Longrightarrow> 
+            P k cfg inp (bins_upd bs (k+1) (Scan_it k inp a x i)) (i+1) \<Longrightarrow> P k cfg inp bs i"
+  assumes pass: "\<And>k cfg inp bs i x a. \<not> i \<ge> length (items (bs ! k)) \<Longrightarrow> x = items (bs ! k) ! i \<Longrightarrow>
+            next_symbol x = Some a \<Longrightarrow> is_terminal cfg a \<Longrightarrow> \<not> k < length inp \<Longrightarrow>
+            P k cfg inp bs (i+1) \<Longrightarrow> P k cfg inp bs i"
+  assumes predict: "\<And>k cfg inp bs i x a. \<not> i \<ge> length (items (bs ! k)) \<Longrightarrow> x = items (bs ! k) ! i \<Longrightarrow>
+            next_symbol x = Some a \<Longrightarrow> \<not> is_terminal cfg a \<Longrightarrow> 
+            P k cfg inp (bins_upd bs k (Predict_it k cfg a)) (i+1) \<Longrightarrow> P k cfg inp bs i"
+  shows "P k cfg inp bs i"
+(*<*)
+  sorry
+(*>*)
+
+lemma wellformed_bins_\<pi>_it':
+  assumes "(k, cfg, inp, bs) \<in> wellformed_bins" 
+  shows "(k, cfg, inp, \<pi>_it' k cfg inp bs i) \<in> wellformed_bins"
+(*<*)
+  sorry
+(*>*)
+
+lemma wellformed_bins_\<pi>_it:
+  assumes "(k, cfg, inp, bs) \<in> wellformed_bins" 
+  shows "(k, cfg, inp, \<pi>_it k cfg inp bs) \<in> wellformed_bins"
+(*<*)
+  sorry
+(*>*)
+
+lemma wellformed_bins_\<I>_it:
+  assumes "k \<le> length inp" "wf_cfg cfg"
+  shows "(k, cfg, inp, \<I>_it k cfg inp) \<in> wellformed_bins"
+(*<*)
+  sorry
+(*>*)
+
+lemma wellformed_bins_\<II>_it:
+  "k \<le> length inp \<Longrightarrow> wf_cfg cfg \<Longrightarrow> (k, cfg, inp, \<II>_it cfg inp) \<in> wellformed_bins"
+(*<*)
+  sorry
+(*>*)
+
+lemma wf_bins_\<pi>_it':
+  assumes "(k, cfg, inp, bs) \<in> wellformed_bins" 
+  shows "wf_bins cfg inp (\<pi>_it' k cfg inp bs i)"
+(*<*)
+  sorry
+(*>*)
+
+lemma wf_bins_\<pi>_it:
+  assumes "(k, cfg, inp, bs) \<in> wellformed_bins" 
+  shows "wf_bins cfg inp (\<pi>_it k cfg inp bs)"
+(*<*)
+  sorry
+(*>*)
+
+lemma wf_bins_\<I>_it:
+  assumes "k \<le> length inp" "wf_cfg cfg"
+  shows "wf_bins cfg inp (\<I>_it k cfg inp)"
+(*<*)
+  sorry
+(*>*)
+
+lemma wf_bins_\<II>_it:
+  "wf_cfg cfg \<Longrightarrow> wf_bins cfg inp (\<II>_it cfg inp)"
+(*<*)
+  sorry
+(*>*)
+
+section \<open>List to set\<close>
+
+lemma Init_it_eq_Init:
+  "bins_items (Init_it cfg inp) = Init cfg"
+(*<*)
+  sorry
+(*>*)
+
+lemma Scan_it_sub_Scan:
+  assumes "wf_bins cfg inp bs" "bins_items bs \<subseteq> I" "x \<in> set (items (bs ! k))"
+  assumes "k < length bs" "k < length inp"
+  assumes "next_symbol x = Some a"
+  shows "set (items (Scan_it k inp a x pre)) \<subseteq> Scan k inp I"
+(*<*)
+  sorry
+(*>*)
+
+lemma Predict_it_sub_Predict:
+  assumes "wf_bins cfg inp bs" "bins_items bs \<subseteq> I" "x \<in> set (items (bs ! k))" "k < length bs"
+  assumes "next_symbol x = Some X"
+  shows "set (items (Predict_it k cfg X)) \<subseteq> Predict k cfg I"
+(*<*)
+  sorry
+(*>*)
+
+lemma Complete_it_sub_Complete:
+  assumes "wf_bins cfg inp bs" "bins_items bs \<subseteq> I" "y \<in> set (items (bs ! k))" "k < length bs"
+  assumes "next_symbol y = None"
+  shows "set (items (Complete_it k y bs red)) \<subseteq> Complete k I"
+(*<*)
+  sorry
+(*>*)
+
+lemma \<pi>_it'_sub_\<pi>:
+  assumes "(k, cfg, inp, bs) \<in> wellformed_bins"
+  assumes "bins_items bs \<subseteq> I"
+  shows "bins_items (\<pi>_it' k cfg inp bs i) \<subseteq> \<pi> k cfg inp I"
+(*<*)
+  sorry
+(*>*)
+
+lemma \<pi>_it_sub_\<pi>:
+  assumes "(k, cfg, inp, bs) \<in> wellformed_bins"
+  assumes "bins_items bs \<subseteq> I"
+  shows "bins_items (\<pi>_it k cfg inp bs) \<subseteq> \<pi> k cfg inp I"
+(*<*)
+  sorry
+(*>*)
+
+lemma \<I>_it_sub_\<I>:
+  assumes "k \<le> length inp" "wf_cfg cfg"
+  shows "bins_items (\<I>_it k cfg inp) \<subseteq> \<I> k cfg inp"
+(*<*)
+  sorry
+(*>*)
+
+lemma \<II>_it_sub_\<II>:
+  "wf_cfg cfg \<Longrightarrow> bins_items (\<II>_it cfg inp) \<subseteq> \<II> cfg inp"
+(*<*)
+  sorry
+(*>*)
+
+section \<open>Soundness\<close>
+
+lemma sound_Scan_it:
+  assumes "wf_bins cfg inp bs" "bins_items bs \<subseteq> I" "x \<in> set (items (bs ! k))" "k < length bs" "k < length inp"
+  assumes "next_symbol x = Some a" "wf_items cfg inp I" "sound_items cfg inp I"
+  shows "sound_items cfg inp (set (items (Scan_it k inp a x i)))"
+(*<*)
+  sorry
+(*>*)
+
+lemma sound_Predict_it:
+  assumes "wf_bins cfg inp bs" "bins_items bs \<subseteq> I" "x \<in> set (items (bs ! k))" "k < length bs"
+  assumes "next_symbol x = Some X" "sound_items cfg inp I"
+  shows "sound_items cfg inp (set (items (Predict_it k cfg X)))"
+(*<*)
+  sorry
+(*>*)
+
+lemma sound_Complete_it:
+  assumes "wf_bins cfg inp bs" "bins_items bs \<subseteq> I" "y \<in> set (items (bs ! k))" "k < length bs"
+  assumes "next_symbol y = None" "wf_items cfg inp I" "sound_items cfg inp I"
+  shows "sound_items cfg inp (set (items (Complete_it k y bs i)))"
+(*<*)
+  sorry
+(*>*)
+
+lemma sound_\<pi>_it':
+  assumes "(k, cfg, inp, bs) \<in> wellformed_bins"
+  assumes "sound_items cfg inp (bins_items bs)"
+  shows "sound_items cfg inp (bins_items (\<pi>_it' k cfg inp bs i))"
+(*<*)
+  sorry
+(*>*)
+
+lemma sound_\<pi>_it:
+  assumes "(k, cfg, inp, bs) \<in> wellformed_bins"
+  assumes "sound_items cfg inp (bins_items bs)"
+  shows "sound_items cfg inp (bins_items (\<pi>_it k cfg inp bs))"
+(*<*)
+  sorry
+(*>*)
+
+section \<open>Set to list\<close>
+
+lemma impossible_complete_item:
+  assumes "wf_cfg cfg" "wf_item cfg inp x" "sound_item cfg inp x"
+  assumes "is_complete x"  "item_origin x = k" "item_end x = k" "nonempty_derives cfg"
+  shows False
+(*<*)
+  sorry
+(*>*)
+
+lemma Complete_Un_eq_terminal:
+  assumes "next_symbol z = Some a" "is_terminal cfg a" "wf_items cfg inp I" "wf_item cfg inp z" "wf_cfg cfg"
+  shows "Complete k (I \<union> {z}) = Complete k I"
+(*<*)
+  sorry
+(*>*)
+
+lemma Complete_Un_eq_nonterminal:
+  assumes "next_symbol z = Some a" "is_nonterminal cfg a" "sound_items cfg inp I" "item_end z = k"
+  assumes "wf_items cfg inp I" "wf_item cfg inp z" "wf_cfg cfg" "nonempty_derives cfg"
+  shows "Complete k (I \<union> {z}) = Complete k I"
+(*<*)
+  sorry
+(*>*)
+
+lemma Complete_bins_upto_eq_bins:
+  assumes "wf_bins cfg inp bs" "k < length bs" "i \<ge> length (items (bs ! k))"
+  shows "Complete k (bins_items_upto bs k i) = Complete k (bins_items bs)"
+(*<*)
+  sorry
+(*>*)
+
+lemma Complete_sub_bins_Un_Complete_it:
+  assumes "Complete k I \<subseteq> bins_items bs" "I \<subseteq> bins_items bs" "is_complete z" "wf_bins cfg inp bs" "wf_item cfg inp z"
+  shows "Complete k (I \<union> {z}) \<subseteq> bins_items bs \<union> set (items (Complete_it k z bs red))"
+(*<*)
+  sorry
+(*>*)
+
+lemma \<pi>_it'_mono:
+  assumes "(k, cfg, inp, bs) \<in> wellformed_bins"
+  shows "bins_items bs \<subseteq> bins_items (\<pi>_it' k cfg inp bs i)"
+(*<*)
+  sorry
+(*>*)
+
+lemma \<pi>_step_sub_\<pi>_it':
+  assumes "(k, cfg, inp, bs) \<in> wellformed_bins"
+  assumes "\<pi>_step k cfg inp (bins_items_upto bs k i) \<subseteq> bins_items bs"
+  assumes "sound_items cfg inp (bins_items bs)" "is_word cfg inp" "nonempty_derives cfg"
+  shows "\<pi>_step k cfg inp (bins_items bs) \<subseteq> bins_items (\<pi>_it' k cfg inp bs i)"
+(*<*)
+  sorry
+(*>*)
+
+lemma \<pi>_step_sub_\<pi>_it:
+  assumes "(k, cfg, inp, bs) \<in> wellformed_bins"
+  assumes "\<pi>_step k cfg inp (bins_items_upto bs k 0) \<subseteq> bins_items bs"
+  assumes "sound_items cfg inp (bins_items bs)" "is_word cfg inp" "nonempty_derives cfg"
+  shows "\<pi>_step k cfg inp (bins_items bs) \<subseteq> bins_items (\<pi>_it k cfg inp bs)"
+(*<*)
+  sorry
+(*>*)
+
+lemma \<pi>_it'_bins_items_eq:
+  assumes "(k, cfg, inp, as) \<in> wellformed_bins"
+  assumes "bins_eq_items as bs" "wf_bins cfg inp as"
+  shows "bins_eq_items (\<pi>_it' k cfg inp as i) (\<pi>_it' k cfg inp bs i)"
+(*<*)
+  sorry
+(*>*)
+
+lemma \<pi>_it'_idem:
+  assumes "(k, cfg, inp, bs) \<in> wellformed_bins"
+  assumes "i \<le> j" "sound_items cfg inp (bins_items bs)" "nonempty_derives cfg"
+  shows "bins_items (\<pi>_it' k cfg inp (\<pi>_it' k cfg inp bs i) j) = bins_items (\<pi>_it' k cfg inp bs i)"
+(*<*)
+  sorry
+(*>*)
+
+lemma \<pi>_it_idem:
+  assumes "(k, cfg, inp, bs) \<in> wellformed_bins"
+  assumes "sound_items cfg inp (bins_items bs)" "nonempty_derives cfg"
+  shows "bins_items (\<pi>_it k cfg inp (\<pi>_it k cfg inp bs)) = bins_items (\<pi>_it k cfg inp bs)"
+(*<*)
+  sorry
+(*>*)
+
+lemma funpower_\<pi>_step_sub_\<pi>_it:
+  assumes "(k, cfg, inp, bs) \<in> wellformed_bins"
+  assumes "\<pi>_step k cfg inp (bins_items_upto bs k 0) \<subseteq> bins_items bs" "sound_items cfg inp (bins_items bs)"
+  assumes "is_word cfg inp" "nonempty_derives cfg"
+  shows "funpower (\<pi>_step k cfg inp) n (bins_items bs) \<subseteq> bins_items (\<pi>_it k cfg inp bs)"
+(*<*)
+  sorry
+(*>*)
+
+lemma \<pi>_sub_\<pi>_it:
+  assumes "(k, cfg, inp, bs) \<in> wellformed_bins"
+  assumes "\<pi>_step k cfg inp (bins_items_upto bs k 0) \<subseteq> bins_items bs" "sound_items cfg inp (bins_items bs)"
+  assumes "is_word cfg inp" "nonempty_derives cfg"
+  shows "\<pi> k cfg inp (bins_items bs) \<subseteq> bins_items (\<pi>_it k cfg inp bs)"
+(*<*)
+  sorry
+(*>*)
+
+lemma \<I>_sub_\<I>_it:
+  assumes "k \<le> length inp" "wf_cfg cfg"
+  assumes "is_word cfg inp" "nonempty_derives cfg"
+  shows "\<I> k cfg inp \<subseteq> bins_items (\<I>_it k cfg inp)"
+(*<*)
+  sorry
+(*>*)
+
+lemma \<II>_sub_\<II>_it:
+  assumes "wf_cfg cfg" "is_word cfg inp" "nonempty_derives cfg"
+  shows "\<II> cfg inp \<subseteq> bins_items (\<II>_it cfg inp)"
+(*<*)
+  sorry
+(*>*)
+
+section \<open>Main Theorem\<close>
+
+definition earley_recognized_it :: "'a bins \<Rightarrow> 'a cfg \<Rightarrow> 'a sentence \<Rightarrow> bool" where
+  "earley_recognized_it I cfg inp = (\<exists>x \<in> set (items (I ! length inp)). is_finished cfg inp x)"
+
+theorem earley_recognized_it_iff_earley_recognized:
+  assumes "wf_cfg cfg" "is_word cfg inp" "nonempty_derives cfg"
+  shows "earley_recognized_it (\<II>_it cfg inp) cfg inp \<longleftrightarrow> earley_recognized (\<II> cfg inp) cfg inp"
+(*<*)
+  sorry
+(*>*)
+
+corollary correctness_list:
+  assumes "wf_cfg cfg" "is_word cfg inp" "nonempty_derives cfg"
+  shows "earley_recognized_it (\<II>_it cfg inp) cfg inp \<longleftrightarrow> derives cfg [\<SS> cfg] inp"
+(*<*)
+  sorry
+(*>*)
 
 (*<*)
 end
