05_Earley_Parser.thy
@@ -1,12 +1,482 @@
 (*<*)
 theory "05_Earley_Parser"
   imports
-    "../Examples"
+    "04_Earley_Recognizer"
+    "HOL-Library.Monad_Syntax"
     "HOL-Library.LaTeXsugar"
 begin
 (*>*)
 
-chapter\<open>Earley Parser\<close>
+chapter\<open>Earley Parser Implementation\<close>
+
+section \<open>Pointer lemmas\<close>
+
+definition predicts :: "'a item \<Rightarrow> bool" where
+  "predicts x \<longleftrightarrow> item_origin x = item_end x \<and> item_dot x = 0"
+
+definition scans :: "'a sentence \<Rightarrow> nat \<Rightarrow> 'a item \<Rightarrow> 'a item \<Rightarrow> bool" where
+  "scans inp k x y \<longleftrightarrow> y = inc_item x k \<and> (\<exists>a. next_symbol x = Some a \<and> inp!(k-1) = a)"
+
+definition completes :: "nat \<Rightarrow> 'a item \<Rightarrow> 'a item \<Rightarrow> 'a item \<Rightarrow> bool" where
+  "completes k x y z \<longleftrightarrow> y = inc_item x k \<and> is_complete z \<and> item_origin z = item_end x \<and>
+    (\<exists>N. next_symbol x = Some N \<and> N = item_rule_head z)"
+
+definition sound_null_ptr :: "'a entry \<Rightarrow> bool" where
+  "sound_null_ptr e = (pointer e = Null \<longrightarrow> predicts (item e))"
+
+definition sound_pre_ptr :: "'a sentence \<Rightarrow> 'a bins \<Rightarrow> nat \<Rightarrow> 'a entry \<Rightarrow> bool" where
+  "sound_pre_ptr inp bs k e = (\<forall>pre. pointer e = Pre pre \<longrightarrow>
+    k > 0 \<and> pre < length (bs!(k-1)) \<and> scans inp k (item (bs!(k-1)!pre)) (item e))"
+
+definition sound_prered_ptr :: "'a bins \<Rightarrow> nat \<Rightarrow> 'a entry \<Rightarrow> bool" where
+  "sound_prered_ptr bs k e = (\<forall>p ps k' pre red. pointer e = PreRed p ps \<and> (k', pre, red) \<in> set (p#ps) \<longrightarrow>
+    k' < k \<and> pre < length (bs!k') \<and> red < length (bs!k) \<and> completes k (item (bs!k'!pre)) (item e) (item (bs!k!red)))"
+
+definition sound_ptrs :: "'a sentence \<Rightarrow> 'a bins \<Rightarrow> bool" where
+  "sound_ptrs inp bs = (\<forall>k < length bs. \<forall>e \<in> set (bs!k).
+    sound_null_ptr e \<and>
+    sound_pre_ptr inp bs k e \<and>
+    sound_prered_ptr bs k e)"
+
+definition mono_red_ptr :: "'a bins \<Rightarrow> bool" where
+  "mono_red_ptr bs = (\<forall>k < length bs. \<forall>i < length (bs!k).
+    \<forall>k' pre red ps. pointer (bs!k!i) = PreRed (k', pre, red) ps \<longrightarrow> red < i)"
+
+lemma sound_ptrs_bin_upd:
+  assumes "sound_ptrs inp bs" "k < length bs" "es = bs!k" "distinct (items es)"
+  assumes "sound_null_ptr e" "sound_pre_ptr inp bs k e" "sound_prered_ptr bs k e"
+  shows "sound_ptrs inp (bs[k := bin_upd e es])"
+(*<*)
+  sorry
+(*>*)
+
+lemma mono_red_ptr_bin_upd:
+  assumes "mono_red_ptr bs" "k < length bs" "es = bs!k" "distinct (items es)"
+  assumes "\<forall>k' pre red ps. pointer e = PreRed (k', pre, red) ps \<longrightarrow> red < length es"
+  shows "mono_red_ptr (bs[k := bin_upd e es])"
+(*<*)
+  sorry
+(*>*)
+
+lemma sound_mono_ptrs_bin_upds:
+  assumes "sound_ptrs inp bs" "mono_red_ptr bs" "k < length bs" "b = bs!k" "distinct (items b)" "distinct (items es)"
+  assumes "\<forall>e \<in> set es. sound_null_ptr e \<and> sound_pre_ptr inp bs k e \<and> sound_prered_ptr bs k e"
+  assumes "\<forall>e \<in> set es. \<forall>k' pre red ps. pointer e = PreRed (k', pre, red) ps \<longrightarrow> red < length b"
+  shows "sound_ptrs inp (bs[k := bin_upds es b]) \<and> mono_red_ptr (bs[k := bin_upds es b])"
+(*<*)
+  sorry
+(*>*)
+
+lemma sound_mono_ptrs_\<pi>_it':
+  assumes "(k, cfg, inp, bs) \<in> wellformed_bins"
+  assumes "sound_ptrs inp bs" "sound_items cfg inp (bins_items bs)"
+  assumes "mono_red_ptr bs"
+  assumes "nonempty_derives cfg" "wf_cfg cfg"
+  shows "sound_ptrs inp (\<pi>_it' k cfg inp bs i) \<and> mono_red_ptr (\<pi>_it' k cfg inp bs i)"
+(*<*)
+  sorry
+(*>*)
+
+lemma sound_mono_ptrs_\<pi>_it:
+  assumes "(k, cfg, inp, bs) \<in> wellformed_bins"
+  assumes "sound_ptrs inp bs" "sound_items cfg inp (bins_items bs)"
+  assumes "mono_red_ptr bs"
+  assumes "nonempty_derives cfg" "wf_cfg cfg"
+  shows "sound_ptrs inp (\<pi>_it k cfg inp bs) \<and> mono_red_ptr (\<pi>_it k cfg inp bs)"
+(*<*)
+  sorry
+(*>*)
+
+lemma sound_ptrs_Init_it:
+  "sound_ptrs inp (Init_it cfg inp)"
+(*<*)
+  sorry
+(*>*)
+
+lemma mono_red_ptr_Init_it:
+  "mono_red_ptr (Init_it cfg inp)"
+(*<*)
+  sorry
+(*>*)
+
+lemma sound_mono_ptrs_\<I>_it:
+  assumes "k \<le> length inp" "wf_cfg cfg" "nonempty_derives cfg" "wf_cfg cfg"
+  shows "sound_ptrs inp (\<I>_it k cfg inp) \<and> mono_red_ptr (\<I>_it k cfg inp)"
+(*<*)
+  sorry
+(*>*)
+
+lemma sound_mono_ptrs_\<II>_it:
+  assumes "wf_cfg cfg" "nonempty_derives cfg"
+  shows "sound_ptrs inp (\<II>_it cfg inp) \<and> mono_red_ptr (\<II>_it cfg inp)"
+(*<*)
+  sorry
+(*>*)
+
+section \<open>Trees and Forests\<close>
+
+datatype 'a tree =
+  Leaf 'a
+  | Branch 'a "'a tree list"
+
+fun yield_tree :: "'a tree \<Rightarrow> 'a sentence" where
+  "yield_tree (Leaf a) = [a]"
+| "yield_tree (Branch _ ts) = concat (map yield_tree ts)"
+
+fun root_tree :: "'a tree \<Rightarrow> 'a" where
+  "root_tree (Leaf a) = a"
+| "root_tree (Branch N _) = N"
+
+fun wf_rule_tree :: "'a cfg \<Rightarrow> 'a tree \<Rightarrow> bool" where
+  "wf_rule_tree _ (Leaf a) \<longleftrightarrow> True"
+| "wf_rule_tree cfg (Branch N ts) \<longleftrightarrow> (
+    (\<exists>r \<in> set (\<RR> cfg). N = rule_head r \<and> map root_tree ts = rule_body r) \<and>
+    (\<forall>t \<in> set ts. wf_rule_tree cfg t))"
+
+fun wf_item_tree :: "'a cfg \<Rightarrow> 'a item \<Rightarrow> 'a tree \<Rightarrow> bool" where
+  "wf_item_tree cfg _ (Leaf a) \<longleftrightarrow> True"
+| "wf_item_tree cfg x (Branch N ts) \<longleftrightarrow> (
+    N = item_rule_head x \<and> map root_tree ts = take (item_dot x) (item_rule_body x) \<and>
+    (\<forall>t \<in> set ts. wf_rule_tree cfg t))"
+
+definition wf_yield_tree :: "'a sentence \<Rightarrow> 'a item \<Rightarrow> 'a tree \<Rightarrow> bool" where
+  "wf_yield_tree inp x t \<longleftrightarrow> yield_tree t = slice (item_origin x) (item_end x) inp"
+
+datatype 'a forest =
+  FLeaf 'a
+  | FBranch 'a "'a forest list list"
+
+fun combinations :: "'a list list \<Rightarrow> 'a list list" where
+  "combinations [] = [[]]"
+| "combinations (xs#xss) = [ x#cs . x <- xs, cs <- combinations xss ]"
+
+fun trees :: "'a forest \<Rightarrow> 'a tree list" where
+  "trees (FLeaf a) = [Leaf a]"
+| "trees (FBranch N fss) = (
+    let tss = (map (\<lambda>fs. concat (map (\<lambda>f. trees f) fs)) fss) in
+    map (\<lambda>ts. Branch N ts) (combinations tss)
+  )"
+
+section \<open>A single parse tree\<close>
+
+partial_function (option) build_tree' :: "'a bins \<Rightarrow> 'a sentence \<Rightarrow> nat \<Rightarrow> nat \<Rightarrow> 'a tree option" where
+  "build_tree' bs inp k i = (
+    let e = bs!k!i in (
+    case pointer e of
+      Null \<Rightarrow> Some (Branch (item_rule_head (item e)) [])
+    | Pre pre \<Rightarrow> (
+        do {
+          t \<leftarrow> build_tree' bs inp (k-1) pre;
+          case t of
+            Branch N ts \<Rightarrow> Some (Branch N (ts @ [Leaf (inp!(k-1))]))
+          | _ \<Rightarrow> None
+        })
+    | PreRed (k', pre, red) _ \<Rightarrow> (
+        do {
+          t \<leftarrow> build_tree' bs inp k' pre;
+          case t of
+            Branch N ts \<Rightarrow>
+              do {
+                t \<leftarrow> build_tree' bs inp k red;
+                Some (Branch N (ts @ [t]))
+              }
+          | _ \<Rightarrow> None
+        })
+  ))"
+
+definition build_tree :: "'a cfg \<Rightarrow> 'a sentence \<Rightarrow> 'a bins \<Rightarrow> 'a tree option" where
+  "build_tree cfg inp bs = (
+    let k = length bs - 1 in (
+    case filter_with_index (\<lambda>x. is_finished cfg inp x) (items (bs!k)) of
+      [] \<Rightarrow> None
+    | (_, i)#_ \<Rightarrow> build_tree' bs inp k i
+  ))"
+
+
+definition wellformed_tree_ptrs :: "('a bins \<times> 'a sentence \<times> nat \<times> nat) set" where
+  "wellformed_tree_ptrs = {
+    (bs, inp, k, i) | bs inp k i.
+      sound_ptrs inp bs \<and>
+      mono_red_ptr bs \<and>
+      k < length bs \<and>
+      i < length (bs!k)
+  }"
+
+fun build_tree'_measure :: "('a bins \<times> 'a sentence \<times> nat \<times> nat) \<Rightarrow> nat" where
+  "build_tree'_measure (bs, inp, k, i) = foldl (+) 0 (map length (take k bs)) + i"
+
+lemma wellformed_tree_ptrs_pre:
+  assumes "(bs, inp, k, i) \<in> wellformed_tree_ptrs"
+  assumes "e = bs!k!i" "pointer e = Pre pre"
+  shows "(bs, inp, (k-1), pre) \<in> wellformed_tree_ptrs"
+(*<*)
+  sorry
+(*>*)
+
+lemma wellformed_tree_ptrs_prered_pre:
+  assumes "(bs, inp, k, i) \<in> wellformed_tree_ptrs"
+  assumes "e = bs!k!i" "pointer e = PreRed (k', pre, red) ps"
+  shows "(bs, inp, k', pre) \<in> wellformed_tree_ptrs"
+(*<*)
+  sorry
+(*>*)
+
+lemma wellformed_tree_ptrs_prered_red:
+  assumes "(bs, inp, k, i) \<in> wellformed_tree_ptrs"
+  assumes "e = bs!k!i" "pointer e = PreRed (k', pre, red) ps"
+  shows "(bs, inp, k, red) \<in> wellformed_tree_ptrs"
+(*<*)
+  sorry
+(*>*)
+
+lemma build_tree'_induct:
+  assumes "(bs, inp, k, i) \<in> wellformed_tree_ptrs"
+  assumes "\<And>bs inp k i.
+    (\<And>e pre. e = bs!k!i \<Longrightarrow> pointer e = Pre pre \<Longrightarrow> P bs inp (k-1) pre) \<Longrightarrow>
+    (\<And>e k' pre red ps. e = bs!k!i \<Longrightarrow> pointer e = PreRed (k', pre, red) ps \<Longrightarrow> P bs inp k' pre) \<Longrightarrow>
+    (\<And>e k' pre red ps. e = bs!k!i \<Longrightarrow> pointer e = PreRed (k', pre, red) ps \<Longrightarrow> P bs inp k red) \<Longrightarrow>
+    P bs inp k i" 
+  shows "P bs inp k i"
+(*<*)
+  sorry
+(*>*)
+
+lemma build_tree'_termination:
+  assumes "(bs, inp, k, i) \<in> wellformed_tree_ptrs"
+  shows "\<exists>N ts. build_tree' bs inp k i = Some (Branch N ts)"
+(*<*)
+  sorry
+(*>*)
+
+lemma wf_item_tree_build_tree':
+  assumes "(bs, inp, k, i) \<in> wellformed_tree_ptrs"
+  assumes "wf_bins cfg inp bs"
+  assumes "k < length bs" "i < length (bs!k)"
+  assumes "build_tree' bs inp k i = Some t"
+  shows "wf_item_tree cfg (item (bs!k!i)) t"
+(*<*)
+  sorry
+(*>*)
+
+lemma wf_yield_tree_build_tree':
+  assumes "(bs, inp, k, i) \<in> wellformed_tree_ptrs"
+  assumes "wf_bins cfg inp bs"
+  assumes "k < length bs" "i < length (bs!k)" "k \<le> length inp"
+  assumes "build_tree' bs inp k i = Some t"
+  shows "wf_yield_tree inp (item (bs!k!i)) t"
+(*<*)
+  sorry
+(*>*)
+
+theorem wf_rule_root_yield_tree_build_tree:
+  assumes "wf_bins cfg inp bs" "sound_ptrs inp bs" "mono_red_ptr bs" "length bs = length inp + 1"
+  assumes "build_tree cfg inp bs = Some t"
+  shows "wf_rule_tree cfg t \<and> root_tree t = \<SS> cfg \<and> yield_tree t = inp"
+(*<*)
+  sorry
+(*>*)
+
+corollary wf_rule_root_yield_tree_build_tree_\<II>_it:
+  assumes "wf_cfg cfg" "nonempty_derives cfg"
+  assumes "build_tree cfg inp (\<II>_it cfg inp) = Some t"
+  shows "wf_rule_tree cfg t \<and> root_tree t = \<SS> cfg \<and> yield_tree t = inp"
+(*<*)
+  sorry
+(*>*)
+
+theorem correctness_build_tree_\<II>_it:
+  assumes "wf_cfg cfg" "is_word cfg inp" "nonempty_derives cfg"
+  shows "(\<exists>t. build_tree cfg inp (\<II>_it cfg inp) = Some t) \<longleftrightarrow> derives cfg [\<SS> cfg] inp"
+(*<*)
+  sorry
+(*>*)
+
+section \<open>Parse trees\<close>
+
+fun insert_group :: "('a \<Rightarrow> 'k) \<Rightarrow> ('a \<Rightarrow> 'v) \<Rightarrow> 'a \<Rightarrow> ('k \<times> 'v list) list \<Rightarrow> ('k \<times> 'v list) list" where
+  "insert_group K V a [] = [(K a, [V a])]"
+| "insert_group K V a ((k, vs)#xs) = (
+    if K a = k then (k, V a # vs) # xs
+    else (k, vs) # insert_group K V a xs  
+  )"
+
+fun group_by :: "('a \<Rightarrow> 'k) \<Rightarrow> ('a \<Rightarrow> 'v) \<Rightarrow> 'a list \<Rightarrow> ('k \<times> 'v list) list" where
+  "group_by K V [] = []"
+| "group_by K V (x#xs) = insert_group K V x (group_by K V xs)"
+
+(*<*)
+lemma [partial_function_mono]:
+  "monotone option.le_fun option_ord
+    (\<lambda>f. map_option concat (those (map (\<lambda>((k', pre), reds).
+      f ((((r, s), k'), pre), {pre}) \<bind>
+        (\<lambda>pres. those (map (\<lambda>red. f ((((r, s), t), red), b \<union> {red})) reds) \<bind>
+          (\<lambda>rss. those (map (\<lambda>f. case f of FBranch N fss \<Rightarrow> Some (FBranch N (fss @ [concat rss])) | _ \<Rightarrow> None) pres))))
+    xs)))"
+  sorry
+(*>*)
+
+partial_function (option) build_trees' :: "'a bins \<Rightarrow> 'a sentence \<Rightarrow> nat \<Rightarrow> nat \<Rightarrow> nat set \<Rightarrow> 'a forest list option" where
+  "build_trees' bs inp k i I = (
+    let e = bs!k!i in (
+    case pointer e of
+      Null \<Rightarrow> Some ([FBranch (item_rule_head (item e)) []])
+    | Pre pre \<Rightarrow> (
+        do {
+          pres \<leftarrow> build_trees' bs inp (k-1) pre {pre};
+          those (map (\<lambda>f.
+            case f of
+              FBranch N fss \<Rightarrow> Some (FBranch N (fss @ [[FLeaf (inp!(k-1))]]))
+            | _ \<Rightarrow> None
+          ) pres)
+        })
+    | PreRed p ps \<Rightarrow> (
+        let ps' = filter (\<lambda>(k', pre, red). red \<notin> I) (p#ps) in
+        let gs = group_by (\<lambda>(k', pre, red). (k', pre)) (\<lambda>(k', pre, red). red) ps' in
+        map_option concat (those (map (\<lambda>((k', pre), reds).
+          do {
+            pres \<leftarrow> build_trees' bs inp k' pre {pre};
+            rss \<leftarrow> those (map (\<lambda>red. build_trees' bs inp k red (I \<union> {red})) reds);
+            those (map (\<lambda>f.
+              case f of
+                FBranch N fss \<Rightarrow> Some (FBranch N (fss @ [concat rss]))
+              | _ \<Rightarrow> None
+            ) pres)
+          }
+        ) gs))
+      )
+  ))"
+
+definition build_trees :: "'a cfg \<Rightarrow> 'a sentence \<Rightarrow> 'a bins \<Rightarrow> 'a forest list option" where
+  "build_trees cfg inp bs = (
+    let k = length bs - 1 in
+    let finished = filter_with_index (\<lambda>x. is_finished cfg inp x) (items (bs!k)) in
+    map_option concat (those (map (\<lambda>(_, i). build_trees' bs inp k i {i}) finished))
+  )"
+
+definition wellformed_forest_ptrs :: "('a bins \<times> 'a sentence \<times> nat \<times> nat \<times> nat set) set" where
+  "wellformed_forest_ptrs = {
+    (bs, inp, k, i, I) | bs inp k i I.
+      sound_ptrs inp bs \<and>
+      k < length bs \<and>
+      i < length (bs!k) \<and>
+      I \<subseteq> {0..<length (bs!k)} \<and>
+      i \<in> I
+  }"
+
+fun build_forest'_measure :: "('a bins \<times> 'a sentence \<times> nat \<times> nat \<times> nat set) \<Rightarrow> nat" where
+  "build_forest'_measure (bs, inp, k, i, I) = foldl (+) 0 (map length (take (k+1) bs)) - card I"
+
+lemma wellformed_forest_ptrs_pre:
+  assumes "(bs, inp, k, i, I) \<in> wellformed_forest_ptrs"
+  assumes "e = bs!k!i" "pointer e = Pre pre"
+  shows "(bs, inp, (k-1), pre, {pre}) \<in> wellformed_forest_ptrs"
+(*<*)
+  sorry
+(*>*)
+
+lemma wellformed_forest_ptrs_prered_pre:
+  assumes "(bs, inp, k, i, I) \<in> wellformed_forest_ptrs"
+  assumes "e = bs!k!i" "pointer e = PreRed p ps"
+  assumes "ps' = filter (\<lambda>(k', pre, red). red \<notin> I) (p#ps)"
+  assumes "gs = group_by (\<lambda>(k', pre, red). (k', pre)) (\<lambda>(k', pre, red). red) ps'"
+  assumes "((k', pre), reds) \<in> set gs"
+  shows "(bs, inp, k', pre, {pre}) \<in> wellformed_forest_ptrs"
+(*<*)
+  sorry
+(*>*)
+
+lemma wellformed_forest_ptrs_prered_red:
+  assumes "(bs, inp, k, i, I) \<in> wellformed_forest_ptrs"
+  assumes "e = bs!k!i" "pointer e = PreRed p ps"
+  assumes "ps' = filter (\<lambda>(k', pre, red). red \<notin> I) (p#ps)"
+  assumes "gs = group_by (\<lambda>(k', pre, red). (k', pre)) (\<lambda>(k', pre, red). red) ps'"
+  assumes "((k', pre), reds) \<in> set gs" "red \<in> set reds"
+  shows "(bs, inp, k, red, I \<union> {red}) \<in> wellformed_forest_ptrs"
+(*<*)
+  sorry
+(*>*)
+
+lemma build_trees'_induct:
+  assumes "(bs, inp, k, i, I) \<in> wellformed_forest_ptrs"
+  assumes "\<And>bs inp k i I.
+    (\<And>e pre. e = bs!k!i \<Longrightarrow> pointer e = Pre pre \<Longrightarrow> P bs inp (k-1) pre {pre}) \<Longrightarrow>
+    (\<And>e p ps ps' gs k' pre reds. e = bs!k!i \<Longrightarrow> pointer e = PreRed p ps \<Longrightarrow>
+      ps' = filter (\<lambda>(k', pre, red). red \<notin> I) (p#ps) \<Longrightarrow>
+      gs = group_by (\<lambda>(k', pre, red). (k', pre)) (\<lambda>(k', pre, red). red) ps' \<Longrightarrow>
+      ((k', pre), reds) \<in> set gs \<Longrightarrow> P bs inp k' pre {pre}) \<Longrightarrow>
+    (\<And>e p ps ps' gs k' pre red reds reds'. e = bs!k!i \<Longrightarrow> pointer e = PreRed p ps \<Longrightarrow>
+      ps' = filter (\<lambda>(k', pre, red). red \<notin> I) (p#ps) \<Longrightarrow>
+      gs = group_by (\<lambda>(k', pre, red). (k', pre)) (\<lambda>(k', pre, red). red) ps' \<Longrightarrow>
+      ((k', pre), reds) \<in> set gs \<Longrightarrow> red \<in> set reds \<Longrightarrow> P bs inp k red (I \<union> {red})) \<Longrightarrow>
+    P bs inp k i I" 
+  shows "P bs inp k i I"
+(*<*)
+  sorry
+(*>*)
+
+lemma build_trees'_termination:
+  assumes "(bs, inp, k, i, I) \<in> wellformed_forest_ptrs"
+  shows "\<exists>fs. build_trees' bs inp k i I = Some fs \<and> (\<forall>f \<in> set fs. \<exists>N fss. f = FBranch N fss)"
+(*<*)
+  sorry
+(*>*)
+
+lemma wf_item_tree_build_trees':
+  assumes "(bs, inp, k, i, I) \<in> wellformed_forest_ptrs"
+  assumes "wf_bins cfg inp bs"
+  assumes "k < length bs" "i < length (bs!k)"
+  assumes "build_trees' bs inp k i I = Some fs"
+  assumes "f \<in> set fs"
+  assumes "t \<in> set (trees f)"
+  shows "wf_item_tree cfg (item (bs!k!i)) t"
+(*<*)
+  sorry
+(*>*)
+
+lemma wf_yield_tree_build_trees':
+  assumes "(bs, inp, k, i, I) \<in> wellformed_forest_ptrs"
+  assumes "wf_bins cfg inp bs"
+  assumes "k < length bs" "i < length (bs!k)" "k \<le> length inp"
+  assumes "build_trees' bs inp k i I = Some fs"
+  assumes "f \<in> set fs"
+  assumes "t \<in> set (trees f)"
+  shows "wf_yield_tree inp (item (bs!k!i)) t"
+(*<*)
+  sorry
+(*>*)
+
+theorem wf_rule_root_yield_tree_build_trees:
+  assumes "wf_bins cfg inp bs" "sound_ptrs inp bs" "length bs = length inp + 1"
+  assumes "build_trees cfg inp bs = Some fs" "f \<in> set fs" "t \<in> set (trees f)"
+  shows "wf_rule_tree cfg t \<and> root_tree t = \<SS> cfg \<and> yield_tree t = inp"
+(*<*)
+  sorry
+(*>*)
+
+corollary wf_rule_root_yield_tree_build_trees_\<II>_it:
+  assumes "wf_cfg cfg" "nonempty_derives cfg"
+  assumes "build_trees cfg inp (\<II>_it cfg inp) = Some fs" "f \<in> set fs" "t \<in> set (trees f)"
+  shows "wf_rule_tree cfg t \<and> root_tree t = \<SS> cfg \<and> yield_tree t = inp"
+(*<*)
+  sorry
+(*>*)
+
+theorem soundness_build_trees_\<II>_it:
+  assumes "wf_cfg cfg" "is_word cfg inp" "nonempty_derives cfg"
+  assumes "build_trees cfg inp (\<II>_it cfg inp) = Some fs" "f \<in> set fs" "t \<in> set (trees f)"
+  shows "derives cfg [\<SS> cfg] inp"
+(*<*)
+  sorry
+(*>*)
+
+theorem termination_build_tree_\<II>_it:
+  assumes "wf_cfg cfg" "nonempty_derives cfg" "derives cfg [\<SS> cfg] inp"
+  shows "\<exists>fs. build_trees cfg inp (\<II>_it cfg inp) = Some fs"
+(*<*)
+  sorry
+(*>*)
+
+section \<open>A word on completeness\<close>
 
 (*<*)
 end
