06_Examples.thy
@@ -6,7 +6,136 @@ theory "06_Examples"
 begin
 (*>*)
 
-chapter\<open>Examples\<close>
+chapter \<open>Examples\<close>
+
+section \<open>epsilon free CFG\<close>
+
+definition \<epsilon>_free :: "'a cfg \<Rightarrow> bool" where
+  "\<epsilon>_free cfg \<longleftrightarrow> (\<forall>r \<in> set (\<RR> cfg). rule_body r \<noteq> [])"
+
+lemma \<epsilon>_free_impl_non_empty_deriv:
+  "\<epsilon>_free cfg \<Longrightarrow> N \<in> set (\<NN> cfg) \<Longrightarrow> \<not> derives cfg [N] []"
+(*<*)
+  sorry  
+(*>*)
+
+section \<open>Example 1: Addition\<close>
+
+datatype t1 = x | plus
+datatype n1 = S
+datatype s1 = Terminal t1 | Nonterminal n1
+
+definition nonterminals1 :: "s1 list" where
+  "nonterminals1 = [Nonterminal S]"
+
+definition terminals1 :: "s1 list" where
+  "terminals1 = [Terminal x, Terminal plus]"
+
+definition rules1 :: "s1 rule list" where
+  "rules1 = [
+    (Nonterminal S, [Terminal x]),
+    (Nonterminal S, [Nonterminal S, Terminal plus, Nonterminal S])
+  ]"
+
+definition start_symbol1 :: s1 where
+  "start_symbol1 = Nonterminal S"
+
+definition cfg1 :: "s1 cfg" where
+  "cfg1 = CFG nonterminals1 terminals1 rules1 start_symbol1"
+
+definition inp1 :: "s1 list" where
+  "inp1 = [Terminal x, Terminal plus, Terminal x, Terminal plus, Terminal x]"
+
+lemma wf_cfg1:
+  "wf_cfg cfg1"
+(*<*)
+  sorry  
+(*>*)
+
+lemma is_word_inp1:
+  "is_word cfg1 inp1"
+(*<*)
+  sorry  
+(*>*)
+
+lemma nonempty_derives1:
+  "nonempty_derives cfg1"
+(*<*)
+  sorry  
+(*>*)
+
+lemma correctness1:
+  "earley_recognized_it (\<II>_it cfg1 inp1) cfg1 inp1 \<longleftrightarrow> derives cfg1 [\<SS> cfg1] inp1"
+(*<*)
+  sorry  
+(*>*)
+
+fun size_bins :: "'a bins \<Rightarrow> nat" where
+  "size_bins bs = fold (+) (map length bs) 0"
+
+value "\<II>_it cfg1 inp1"
+value "size_bins (\<II>_it cfg1 inp1)"
+value "earley_recognized_it (\<II>_it cfg1 inp1) cfg1 inp1"
+value "build_trees cfg1 inp1 (\<II>_it cfg1 inp1)"
+value "map_option (map trees) (build_trees cfg1 inp1 (\<II>_it cfg1 inp1))"
+value "map_option (foldl (+) 0 \<circ> map length) (map_option (map trees) (build_trees cfg1 inp1 (\<II>_it cfg1 inp1)))"
+
+subsection \<open>Example 2: Cyclic reduction pointers\<close>
+
+datatype t2 = x
+datatype n2 = A | B
+datatype s2 = Terminal t2 | Nonterminal n2
+
+definition nonterminals2 :: "s2 list" where
+  "nonterminals2 = [Nonterminal A, Nonterminal B]"
+
+definition terminals2 :: "s2 list" where
+  "terminals2 = [Terminal x]"
+
+definition rules2 :: "s2 rule list" where
+  "rules2 = [
+    (Nonterminal B, [Nonterminal A]),
+    (Nonterminal A, [Nonterminal B]),
+    (Nonterminal A, [Terminal x])
+  ]"
+
+definition start_symbol2 :: s2 where
+  "start_symbol2 = Nonterminal A"
+
+definition cfg2 :: "s2 cfg" where
+  "cfg2 = CFG nonterminals2 terminals2 rules2 start_symbol2"
+
+definition inp2 :: "s2 list" where
+  "inp2 = [Terminal x]"
+
+lemma wf_cfg2:
+  "wf_cfg cfg2"
+(*<*)
+  sorry  
+(*>*)
+
+lemma is_word_inp2:
+  "is_word cfg2 inp2"
+(*<*)
+  sorry  
+(*>*)
+
+lemma nonempty_derives2:
+  "nonempty_derives cfg2"
+(*<*)
+  sorry  
+(*>*)
+
+lemma correctness2:
+  "earley_recognized_it (\<II>_it cfg2 inp2) cfg2 inp2 \<longleftrightarrow> derives cfg2 [\<SS> cfg2] inp2"
+(*<*)
+  sorry  
+(*>*)
+
+value "\<II>_it cfg2 inp2"
+value "earley_recognized_it (\<II>_it cfg2 inp2) cfg2 inp2"
+value "build_trees cfg2 inp2 (\<II>_it cfg2 inp2)"
+value "map_option (map trees) (build_trees cfg2 inp2 (\<II>_it cfg2 inp2))"
 
 (*<*)
 end
